src/Hoare.v
@@ -85,6 +85,28 @@ Notation "{< e1 .. e2 , 'PRE' pre 'POST' : rp post 'CRASH' : rc crash >} p1 >> p
    (p2 rxREC)%pred)) .. ))
   (at level 0, p1 at level 60, p2 at level 60, e1 binder, e2 binder, rp at level 0, rc at level 0).
 
+Notation "{< e1 .. e2 , 'PRE' pre 'POST' : ( rp1 , rp2 ) post 'CRASH' : rc crash >} p1 >> p2" :=
+  (forall_helper (fun e1 => .. (forall_helper (fun e2 =>
+   exists idemcrash,
+   forall TF TR (rxOK: _ -> prog TF) (rxREC: _ -> prog TR),
+   corr3
+   (fun done_ crashdone_ =>
+     exists F,
+     F * pre *
+     [[ crash_xform F =p=> F ]] *
+     [[ forall r_,
+        {{ fun done'_ crash'_ => (fun rp1 rp2 => F * post) (fst r_) (snd r_) *
+                                 [[ done'_ = done_ ]] * [[ crash'_ =p=> F * idemcrash ]]
+        }} rxOK r_ ]] *
+     [[ forall r_,
+        {{ fun done'_ crash'_ => (fun rc => F * crash) r_ *
+                                 [[ done'_ = crashdone_ ]] * [[ crash'_ =p=> F * idemcrash ]]
+        }} rxREC r_ ]]
+   )%pred
+   (p1 rxOK)%pred
+   (p2 rxREC)%pred)) .. ))
+  (at level 0, p1 at level 60, p2 at level 60, e1 binder, e2 binder, rp1 at level 0, rp2 at level 0, rc at level 0).
+
 
 Theorem pimpl_ok2:
   forall T pre pre' (pr: prog T),
